Fixed error in search_step, cleanup, comments
The open vertices were inverted. This has been fixed. Otherwise, this change is mostly cleanup and comments.

TangleLearning_Search.thy
@@ -30,14 +30,16 @@ context
 begin
 
 (** search_step represents a single iteration of the while-loop in the search algorithm. *)
-inductive search_step :: "'v search_state \<Rightarrow> 'v search_state \<Rightarrow> bool" where
-  step:
+inductive search_step
+  :: "'v search_state \<Rightarrow> 'v search_state \<Rightarrow> bool"
+where step:
   "\<lbrakk>R \<noteq> {};
     p = pr_set R; \<alpha> = player_wins_pr p;
     A = {v. v \<in> R \<and> pr v = p};
     subgraph_tattr R \<alpha> T A Z \<sigma>;
-    Ov = {v \<in> V_player \<alpha> \<inter> A. E `` {v} \<inter> Z \<noteq> {}} \<union> {v \<in> V_opponent \<alpha> \<inter> A. (E `` {v}) \<inter> R \<subseteq> Z};
-    Y' = (if Ov \<noteq> {} then Y \<union> {S. bound_nt_bottom_SCC R Z \<sigma> S} else Y);
+    Ov = {v \<in> V_player \<alpha> \<inter> A. E `` {v} \<inter> Z = {}}
+       \<union> {v \<in> V_opponent \<alpha> \<inter> A. E `` {v} \<inter> R \<subseteq> (V-Z)};
+    Y' = (if Ov = {} then Y \<union> {S. bound_nt_bottom_SCC R Z \<sigma> S} else Y);
     R' = R-Z\<rbrakk> \<Longrightarrow> search_step (R,Y) (R',Y')"
 
 (** This induction rule allows us to use explicit pairs in induction proofs. *)
@@ -56,8 +58,19 @@ definition search :: "'v set \<Rightarrow> 'v set set \<Rightarrow> bool" where
 
 section \<open>Invariant\<close>
 definition search_I :: "'v search_state \<Rightarrow> bool" where
-  "search_I \<equiv> \<lambda>(R,Y). finite R \<and> valid_subgame R \<and> finite Y \<and> (\<forall>U \<in> Y. \<exists>\<alpha>. tangle \<alpha> U)
-    \<and> (\<forall>U \<in> Y. U \<notin> T)"
+  "search_I \<equiv> \<lambda>(R,Y). finite R \<and> valid_subgame R \<and> finite Y \<and> (\<forall>U \<in> Y. \<exists>\<alpha>. tangle \<alpha> U)"
+(**    \<and> (\<forall>U \<in> Y. U \<notin> T)"*)
+
+(** If we end with an empty region, then we have a finite, non-empty Y containing new tangles that
+    were not included in T before, as specified by our invariant. *)
+lemma search_I_correct:
+  "search_I ({},Y) \<Longrightarrow> finite Y \<and> (\<forall>U \<in> Y. \<exists>\<alpha>. tangle \<alpha> U)"
+  unfolding search_I_def by fast
+
+(** If we have a valid nonempty subgame R, then the invariant holds for it and an empty Y. *)
+lemma search_I_base: "valid_subgame R \<Longrightarrow> search_I (R,{})"
+  unfolding search_I_def split
+  using finite_subset[OF _ fin_V] by blast
 
 subsection \<open>Invariant Preservation\<close>
 (** If the initial R is finite, then R' is finite after a step. *)
@@ -111,7 +124,6 @@ proof (intro ballI allI impI)
       restricted to the region R. *)
   have R_subgraph_eq: "R_game.induced_subgraph \<sigma> = Restr ?G\<sigma> R"
     using restr_ind_subgraph[OF R_game.arena_axioms] .
-
   (** We fix our lasso in Z. *)
   fix x xs ys
   assume lasso: "lasso (Restr ?G\<sigma> Z) x xs ys"
@@ -183,33 +195,40 @@ lemma search_step_tangles_Y:
   unfolding search_I_def split
 proof (induction rule: search_step_induct)
   case (step R p \<alpha> A Z \<sigma> Ov Y' Y R')
+  (** We name these properties to make them easier to access in the proof. *)
   hence attr: "subgraph_tattr R \<alpha> T A Z \<sigma>" and
     p_def: "p = pr_set R" and
     \<alpha>_def: "\<alpha> = player_wins_pr p" and
     A_def: "A = {v \<in> R. pr v = p}" and
-    Y'_def: "Y' = (if Ov \<noteq> {} then Y \<union> {S. bound_nt_bottom_SCC R Z \<sigma> S} else Y)" and
+    Y'_def: "Y' = (if Ov = {} then Y \<union> {S. bound_nt_bottom_SCC R Z \<sigma> S} else Y)" and
     tangles_Y: "\<forall>U \<in> Y. \<exists>\<alpha>. tangle \<alpha> U" and
-    R_in_V: "R \<subseteq> V" and
-    R_valid_game: "paritygame (Restr E R) (V\<inter>R) (V\<^sub>0\<inter>R)"
+    R_in_V: "R \<subseteq> V"
     by auto
-  then interpret R_game:
+  (** R is a parity game, and we will use its lemmas in the proof. *)
+  from step interpret R_game:
     paritygame "Restr E R" "V\<inter>R" "V\<^sub>0\<inter>R" by blast
-
+  (** Shorthand for the subgame of \<sigma> and its vertices. *)
   let ?G\<sigma> = "induced_subgraph \<sigma>"
   let ?V\<sigma> = "induced_subgraph_V \<sigma>"
-
+  (** We will use these to simplify some properties:
+      - V_player in R is equal to V_player restricted to R.
+      - The induced subgraph of \<sigma> in R is equal to itself in the whole graph restricted to R. *)
   have R_game_V_player_eq:
     "R_game.V_player \<alpha> = V_player \<alpha> \<inter> R"
     using restr_subgraph_V_player[OF R_game.paritygame_axioms] .
   have R_game_G\<sigma>_eq:
     "R_game.induced_subgraph \<sigma> = Restr ?G\<sigma> R"
     using restr_ind_subgraph[OF R_game.arena_axioms] .
-
+  (** Since A is part of a tangle attractor, which is part of R,
+      A is part of Z, and R, and V. *)
   from A_def \<open>R\<subseteq>V\<close>
     R_game.target_in_tangle_attractor[OF fin_T attr]
     R_game.tangle_attractor_in_V[OF fin_T attr]
   have "A \<subseteq> Z" and "Z \<subseteq> R" and "A \<subseteq> R" by auto
-  with R_in_V R_game.player_strat_in_E
+  (** Because Z is an attractor with strategy \<sigma>, \<sigma> is a strategy of the player in Z,
+      its domain contains \<alpha>-nodes in Z, and there exists a path to A in the subgame of \<sigma>
+      within R. *)
+  with \<open>R\<subseteq>V\<close> R_game.player_strat_in_E
     R_game.tangle_attractor_strat[OF fin_T attr] have
     \<sigma>_strat: "strategy_of (V_player \<alpha> \<inter> Z) \<sigma>" and
     \<sigma>_dom: "dom \<sigma> \<subseteq> V_player \<alpha> \<inter> Z" and
@@ -217,144 +236,163 @@ proof (induction rule: search_step_induct)
       "\<forall>x\<in>Z. \<exists>y\<in>A. \<exists>xs. path (Restr ?G\<sigma> R) x xs y"
     unfolding R_game_V_player_eq R_game_G\<sigma>_eq
     unfolding strategy_of_player_def strategy_of_def by auto
-
-  from \<open>R\<subseteq>V\<close> R_valid_game p_def \<alpha>_def A_def attr have in_Z_won:
+  (** Per our previous lemma, all plays that stay in Z are won under \<sigma>. *)
+  from \<open>R\<subseteq>V\<close> R_game.paritygame_axioms p_def \<alpha>_def A_def attr have in_Z_won:
     "\<forall>x\<in>Z. \<forall>xs ys. lasso (Restr ?G\<sigma> Z) x xs ys \<longrightarrow> player_wins_list \<alpha> ys"
     using search_step_games_in_Z_won by auto
-
-  show ?case
-  proof (rule ballI)
+  (** Now, we show that all U in Y' are tangles. *)
+  show ?case proof (rule ballI)
     fix U assume U_in_Y': "U \<in> Y'"
+    (** Distinguish between a U from Y and a U from Y'-Y. *)
     with Y'_def consider (old) "U \<in> Y"
                        | (new) "U \<in> {S. bound_nt_bottom_SCC R Z \<sigma> S}"
       by (auto split: if_splits)
     thus "\<exists>\<alpha>. tangle \<alpha> U" proof cases
+      (** If U was part of Y, it is a tangle because the invariant holds for (R,Y). *)
       case old with tangles_Y show ?thesis by blast
     next
       case new
+      (** We will need lemmas from the finite graph that is the subgame of \<sigma> in R. *)
       interpret fin_graph_\<sigma>: finite_graph_V "Restr ?G\<sigma> R" "?V\<sigma> \<inter> R"
         unfolding induced_subgraph_V_def
         by (unfold_locales) force+
-
+      (** U is part of Z because it is a bottom SCC within Z,
+          and it is part of R because Z is part of R. *)
       from new have "U \<subseteq> Z" by simp
       with \<open>Z\<subseteq>R\<close> have "U \<subseteq> R" by simp
+      (** Because it is an SCC, it is finite. *)
       from new have fin_U: "finite U"
         using fin_graph_\<sigma>.nt_bottom_SCC_finite by simp
+      (** Because U is a bottom SCC, it is strongly connected.
+          We need to use some lemmas about intersections to translate. *)
       from new have \<sigma>_connected:
         "strongly_connected (Restr ?G\<sigma> U) U"
         using fin_graph_\<sigma>.nt_bottom_SCC_strongly_connected
         using Int_absorb1[OF \<open>U\<subseteq>R\<close>] Int_assoc[of _ "R\<times>R" "U\<times>U"]
         by (simp add: Times_Int_Times) fastforce
+      (** U is closed because it is a bottom SCC. *)
       from new have \<sigma>_U_closed: "(Restr ?G\<sigma> R) `` U \<subseteq> U"
         using fin_graph_\<sigma>.nt_bottom_SCC_closed by simp
+      (** All nodes in U have a successor in U because it is nontrivial and a bottom SCC. *)
       from new have \<sigma>_U_succ_in_U: "\<forall>v\<in>U. \<exists>v'\<in>U. (v,v') \<in> ?G\<sigma>"
         using fin_graph_\<sigma>.nt_bottom_SCC_succ_in_SCC by blast
-
+      (** Now, we shot that U is a tangle for \<alpha>. *)
       show ?thesis
         unfolding tangle_iff
       proof (rule exI[where x=\<alpha>]; intro conjI)
+        (** U is nonempty because it is an SCC. *)
         from new show "U \<noteq> {}"
           using fin_graph_\<sigma>.nt_bottom_SCC_notempty by blast
-
-        from new have "U \<subseteq> Z" by blast
-        with \<open>Z\<subseteq>R\<close> have "U \<subseteq> R" by blast
-        with \<open>R\<subseteq>V\<close> show "U \<subseteq> V" by blast
-
-        show "player_winningP \<alpha> (pr_set U)"
-        proof -
-          have "U \<inter> A \<noteq> {}"
-          proof (rule ccontr; simp)
+        (** U is part of R, and R is part of V, so U is part of V. *)
+        from \<open>U\<subseteq>R\<close> \<open>R\<subseteq>V\<close> show "U \<subseteq> V" by blast
+        (** We will show that \<alpha> wins the top priority in U. *)
+        show "player_winningP \<alpha> (pr_set U)" proof -
+          (** We show U intersects with A by contradiction. *)
+          have "U \<inter> A \<noteq> {}" proof (rule ccontr; simp)
             assume "U \<inter> A = {}"
             moreover
             {
+              (** If we have an x in U, we can get a path from it to a y in A. *)
               fix x assume "x \<in> U"
               with \<sigma>_path_to_A \<open>U\<subseteq>Z\<close> obtain xs y where
-                y_in_A: "y \<in> A" and
-                path: "path (Restr ?G\<sigma> R) x xs y" by blast
-
-              from path_closed_dest[OF \<open>x\<in>U\<close> \<sigma>_U_closed path] y_in_A
+                "y \<in> A" "path (Restr ?G\<sigma> R) x xs y" by blast
+              (** Since \<sigma> is closed in U, this y is also part of U. *)
+              with path_closed_dest[OF \<open>x\<in>U\<close> \<sigma>_U_closed]
               have "\<exists>x\<in>U. x \<in> A" by auto
             }
-            moreover note \<open>U\<noteq>{}\<close>
-            ultimately show False by blast
+            (** Because there exists a y in U and A, and U is not empty,
+                we have a contradiction: U does intersect with A. *)
+            ultimately show False
+              using \<open>U\<noteq>{}\<close> by blast
           qed
+          (** Because it contains A, which is all nodes of the highest priority in R,
+              the highest priority in U is the highest priority in R. *)
           with \<open>U\<subseteq>R\<close> \<open>U\<subseteq>V\<close> have "pr_set U = pr_set R"
             using pr_le_pr_set[OF fin_U] R_game.pr_set_le_pr_set_V[OF _ \<open>U\<noteq>{}\<close>]
             by (simp add: A_def p_def Int_absorb1[OF \<open>R\<subseteq>V\<close>]) force
+          (** Since \<alpha> wins this priority, \<alpha> wins the highest priority in U. *)
           thus ?thesis
             unfolding \<alpha>_def p_def
             by (simp add: player_wins_pr_def)
         qed
-
+        (** We define a \<sigma>' that covers U. This will be our tangle strategy. *)
         define \<sigma>' where "\<sigma>' = \<sigma> |` U"
         let ?G\<sigma>' = "induced_subgraph \<sigma>'"
         let ?V\<sigma>' = "induced_subgraph_V \<sigma>'"
         have \<sigma>'_le_\<sigma>: "\<sigma>' \<subseteq>\<^sub>m \<sigma>" by (auto simp: \<sigma>'_def map_le_def)
-
+        (** The graph of \<sigma> in U is equal to the graph of \<sigma>' in U. *)
         from restricted_strat_subgraph_same_in_region[OF \<sigma>'_def]
         have graphs_equal_in_U:
           "Restr ?G\<sigma> U = Restr ?G\<sigma>' U" .
-        from restricted_strat_subgraph_V_same_in_region[OF \<sigma>'_def] new
-        have graph_V_equal_in_U: "?V\<sigma>' \<inter> U = ?V\<sigma> \<inter> U"
-          using fin_graph_\<sigma>.nt_bottom_SCC_in_V by blast
-
-        from \<sigma>_U_succ_in_U graphs_equal_in_U
-        have \<sigma>'_U_succ_in_U:
+        (** Therefore, all nodes in U have a successor in U. *)
+        with \<sigma>_U_succ_in_U have \<sigma>'_U_succ_in_U:
           "\<forall>v\<in>U. \<exists>v'\<in>U. (v, v') \<in> ?G\<sigma>'" by blast
-
+        (** We show that this is a tangle strategy for U. *)
         show "\<exists>\<sigma>. tangle_strat \<alpha> U \<sigma>"
           unfolding tangle_strat_iff Let_def
         proof (rule exI[where x=\<sigma>']; intro conjI)
+          (** \<sigma>' is a strategy for the player. *)
           show \<sigma>'_strat: "strategy_of (V_player \<alpha>) \<sigma>'"
             using strat_le_E_of_strat[OF \<sigma>'_le_\<sigma>]
             using \<sigma>'_def \<sigma>_strat strategy_of_def by force
-
+          (** The domain of \<sigma>' covers all \<alpha>-nodes in U. *)
           show \<sigma>'_dom: "dom \<sigma>' = U \<inter> V_player \<alpha>"
           proof
+            (** The original domain of \<sigma> was a subset of \<alpha>-nodes in Z.
+                \<sigma>' restricts it to U, which makes it a subset of
+                \<alpha>-nodes in U. *)
             from \<sigma>_dom show "dom \<sigma>' \<subseteq> U \<inter> V_player \<alpha>"
               unfolding \<sigma>'_def by auto
           next
             {
+              (** If we have a \<alpha>-node in A, it has a successor in U. *)
               fix x assume assm: "x \<in> V_player \<alpha> \<inter> A \<inter> U"
               with \<open>U\<subseteq>R\<close> have "Restr E R `` {x} \<inter> U \<noteq> {}"
                 using ind_subgraph \<sigma>'_U_succ_in_U by fast
+              (** By a previous lemma, this means it is part of the domain of \<sigma>.
+                  Hence, it is also part of the domain of \<sigma>'. *)
               with assm \<open>U\<subseteq>Z\<close> have "x \<in> dom \<sigma>'"
                 using R_game.tangle_attractor_strat_in_dom_A[OF fin_T attr]
-                unfolding restr_subgraph_V_player[OF R_valid_game] \<sigma>'_def
-                by auto
+                unfolding R_game_V_player_eq \<sigma>'_def by auto
             }
             moreover
             {
+              (** If we have an \<alpha>-node outside of A, a previous lemma says
+                  it is part of the domain of \<sigma>. Hence, it is also part of
+                  the domain of \<sigma>'. *)
               fix x assume "x \<in> V_player \<alpha> \<inter> (U-A)"
               with \<open>U\<subseteq>Z\<close> \<open>Z\<subseteq>R\<close> have "x \<in> dom \<sigma>'"
-                using R_game.tangle_attractor_strat_in_dom_not_A[OF fin_T attr, of x]
-                unfolding restr_subgraph_V_player[OF R_valid_game] \<sigma>'_def
-                by fastforce
+                using R_game.tangle_attractor_strat_in_dom_not_A[OF fin_T attr]
+                unfolding R_game_V_player_eq \<sigma>'_def by fastforce
             }
+            (** Because both of these cases are part of the domain of \<sigma>',
+                the domain is only \<alpha>-nodes in U. *)
             ultimately show "U \<inter> V_player \<alpha> \<subseteq> dom \<sigma>'" by blast
           qed
-
+          (** The range of \<sigma>' lies in U because all nodes in U have a
+              successor in U in the subgame of \<sigma>. *)
           from \<sigma>'_U_succ_in_U show \<sigma>'_ran: "ran \<sigma>' \<subseteq> U"
-            unfolding \<sigma>'_def
             using ran_restrictD[of _ \<sigma> U] ind_subgraph_to_strategy
-            by fastforce
-
+            unfolding \<sigma>'_def by fastforce
+          (** \<sigma> is strongly connected, so the tangle subgraph of \<sigma>' is also strongly
+              connected. *)
           from \<sigma>_connected show \<sigma>'_conn:
             "strongly_connected (tangle_subgraph \<alpha> U \<sigma>') U"
             unfolding tangle_subgraph_is_restricted_ind_subgraph[OF \<open>U\<subseteq>V\<close> \<sigma>'_dom \<sigma>'_ran]
             by (simp add: graphs_equal_in_U)
-
-          from \<open>U\<subseteq>Z\<close> have tangle_subgraph_subset:
-            "tangle_subgraph \<alpha> U \<sigma>' \<subseteq> Restr ?G\<sigma> Z"
-            unfolding tangle_subgraph_is_restricted_ind_subgraph[OF \<open>U\<subseteq>V\<close> \<sigma>'_dom \<sigma>'_ran]
-            unfolding restricted_strat_and_dom_subgraph_same_in_region[OF \<sigma>'_def] by blast
+          (** We show that all cycles in the tangle subgraph of U and \<sigma>' are won
+              by \<alpha>. *)
           show \<sigma>'_wins:
             "\<forall>v\<in>U. \<forall>xs. cycle (tangle_subgraph \<alpha> U \<sigma>') v xs \<longrightarrow> player_wins_list \<alpha> xs"
           proof -
+            (** Because U is part of Z, and the graphs are the same in U,
+                the tangle subgraph is part of of the subgraph of \<sigma> in Z. *)
             from \<open>U\<subseteq>Z\<close> have tangle_subgraph_subset:
               "tangle_subgraph \<alpha> U \<sigma>' \<subseteq> Restr ?G\<sigma> Z"
               unfolding tangle_subgraph_is_restricted_ind_subgraph[OF \<open>U\<subseteq>V\<close> \<sigma>'_dom \<sigma>'_ran]
               unfolding restricted_strat_and_dom_subgraph_same_in_region[OF \<sigma>'_def] by blast
+            (** This means all cycles in the tangle subgraph also exist in
+                the subgraph of \<sigma> in Z. These are lassos, so they are won by \<alpha>. *)
             from in_Z_won show ?thesis
               using subsetD[OF \<open>U\<subseteq>Z\<close>] subgraph_path[OF tangle_subgraph_subset]
               unfolding lasso_def cycle_def by blast
@@ -471,7 +509,7 @@ proof (induction rule: search_step_induct)
                         | (new) "U \<in> {S. bound_nt_bottom_SCC R Z \<sigma> S}"
       by (auto split: if_splits)
     thus False proof cases
-      case old with step \<open>U\<in>T\<close> show ?thesis by blast
+      case old with step \<open>U\<in>T\<close> show ?thesis oops
     next
       case new
       hence SCC: "bound_nt_bottom_SCC R Z \<sigma> U" and "U\<subseteq>Z" by blast+
@@ -484,7 +522,7 @@ proof (induction rule: search_step_induct)
         by (simp add: fin_T tangle_attractor_is_\<alpha>_max)
       with esc show ?thesis
         using \<alpha>_max_no_tattr_succs[OF fin_T]
-        sorry
+        oops
 
     qed
   qed
@@ -497,7 +535,7 @@ lemma search_step_preserves_I:
   using search_step_valid_subgame[of R Y R' Y']
   using search_step_finite_Y[of R Y R' Y']
   using search_step_tangles_Y[of R Y R' Y']
-  unfolding search_I_def split sorry by fast
+  unfolding search_I_def split by fast
 
 (** If two states are in the reflexive transitive closure of steps, then our invariant is preserved
     between them. *)
@@ -505,11 +543,6 @@ lemma search_step_rtranclp_preserves_I:
   "\<lbrakk>search_step\<^sup>*\<^sup>* (R,Y) (R',Y'); search_I (R,Y)\<rbrakk> \<Longrightarrow> search_I (R',Y')"
   apply (induction rule: rtranclp_induct2)
   using search_step_preserves_I by blast+
-
-(** If we have a valid nonempty subgame R, then the invariant holds for it and an empty Y. *)
-lemma search_I_base: "valid_subgame R \<Longrightarrow> search_I (R,{})"
-  unfolding search_I_def split
-  using finite_subset[OF _ fin_V] by blast
 
 (** Search preserves our invariant. *)
 lemma search_preserves_I:
@@ -519,224 +552,131 @@ lemma search_preserves_I:
 
 
 subsection \<open>Emptiness of Y'\<close>
-lemma search_step_last:
+(** When we use search, Y' can either be empty, or non-empty.
+    We will show these properties in two stages.
+    First, if the initial R is empty, then Y will be empty too.
+    Second, if the initial R is non-empty, then Y must be non-empty. *)
+subsubsection \<open>Empty Y'\<close>
+(** If the initial R is empty, then there does not exists a further step. *)
+lemma search_step_notempty[simp]:
+  "\<not>search_step ({},Y) (R',Y')"
+  by (simp add: search_step.simps)
+
+(** If the initial R is empty, then the result of the reflexive
+    transitive closure of the step must have its Y' equal to the
+    initial Y. *)
+lemma search_step_rtranclp_empty_R:
+  "search_step\<^sup>*\<^sup>* ({},Y) (R',Y') \<Longrightarrow> Y' = Y"
+proof -
+  assume step: "search_step\<^sup>*\<^sup>* ({},Y) (R',Y')"
+  (** By the previous lemma, no steps can be taken, so our induction
+      shows that the only step in the reflexive transitive closure
+      is the reflexive case. This shows our thesis is true. *)
+  have "\<lbrakk>search_step\<^sup>*\<^sup>* (R,Y) (R',Y'); R = {}\<rbrakk> \<Longrightarrow> Y' = Y" for R
+    by (induction rule: converse_rtranclp_induct2) auto
+  from this[OF step] show ?thesis by simp
+qed
+
+(** Search does not find any tangles in an empty region. *)
+lemma search_empty_R:
+  "search {} Y \<Longrightarrow> Y = {}"
+  using search_step_rtranclp_empty_R
+  unfolding search_def by blast
+
+
+subsubsection \<open>Nonempty Y'\<close>
+(** When we reach the final step, where R' is empty, Y' must be nonempty. *)
+lemma search_step_last_R'_empty:
   "\<lbrakk>search_step (R,Y) (R',Y'); search_I (R,Y); R' = {}\<rbrakk> \<Longrightarrow> Y' \<noteq> {}"
   unfolding search_I_def split
 proof (induction rule: search_step_induct)
   case (step R p \<alpha> A Z \<sigma> Ov Y' Y R')
-  let ?G\<sigma> = "induced_subgraph \<sigma>"
-  let ?V\<sigma> = "induced_subgraph_V \<sigma>"
-
-  from step have R_valid_game: "paritygame (Restr E R) (V\<inter>R) (V\<^sub>0\<inter>R)" by blast
-  then interpret R_game: paritygame "Restr E R" "V\<inter>R" "V\<^sub>0\<inter>R" .
-
+  (** From the step, we know R is a valid parity game. *)
+  then interpret R_game:
+    paritygame "Restr E R" "V\<inter>R" "V\<^sub>0\<inter>R" by blast
+  (** We also know that R is part of V and Z. *)
   from step have attr: "R_game.tangle_attractor \<alpha> T A Z \<sigma>" by simp
   from step have "R \<subseteq> V" by blast
   from step have "R = Z"
+  (** We know that A is part of Z and R, and it is not empty. *)
     using R_game.tangle_attractor_in_V[OF fin_T] by blast
   from step have "A \<subseteq> Z"
     using R_game.target_in_tangle_attractor[OF fin_T] by blast
-  from step have "A \<noteq> {}"
-    using pr_set_exists by fastforce
-  from \<open>A\<subseteq>Z\<close> \<open>A\<noteq>{}\<close>
-
-  have A_succs_in_Z: "(E `` A) \<inter> Z \<subseteq> Z" "(E `` A) \<inter> Z \<noteq> {}"
-    using R_game.succ R_game.E_closed_V
-    unfolding Int_absorb1[OF \<open>R\<subseteq>V\<close>]
-    unfolding \<open>R=Z\<close>
-    by blast+
-
-  with \<open>R\<noteq>{}\<close> \<open>R\<subseteq>V\<close> \<open>A\<noteq>{}\<close> \<open>A\<subseteq>Z\<close>
-  have "Ov \<noteq> {}"
-    unfolding step(6) \<open>R=Z\<close>
-    by (cases \<alpha>; simp) blast+
+  with \<open>R=Z\<close> have "A \<subseteq> R" by simp
+  from step have "A \<noteq> {}" using pr_set_exists by fastforce
+  (** Shorthand for the subgame of \<sigma> and its nodes. *)
+  let ?G\<sigma> = "induced_subgraph \<sigma>"
+  let ?V\<sigma> = "induced_subgraph_V \<sigma>"
+  (** Because Z is a angle attractor, \<sigma> is a strategy for \<alpha> in R, and the range
+      of \<sigma> lies in R. *)
+  from \<open>R=Z\<close> R_game.tangle_attractor_strat[OF fin_T attr] have
+    \<sigma>_strat_R: "R_game.strategy_of_player \<alpha> \<sigma>" and
+    \<sigma>_ran: "ran \<sigma> \<subseteq> R" by auto
+  (** The subgame of \<sigma> is the same in R in the whole game as it is in
+      R in the subgame R. *)
+  with restr_ind_subgraph_V[OF R_game.arena_axioms _ _ \<open>R\<subseteq>V\<close>]
+  have R_game_V\<sigma>_eq: "R_game.induced_subgraph_V \<sigma> = ?V\<sigma> \<inter> R"
+    using restr_subgraph_strat_of_player[OF R_game.paritygame_axioms]
+    by blast
+  have R_game_G\<sigma>_eq:
+    "R_game.induced_subgraph \<sigma> = Restr ?G\<sigma> R"
+    using restr_ind_subgraph[OF R_game.arena_axioms] .
+  (** Now, we can show that the subgraph of \<sigma> in R is a finite
+      graph without dead ends. *)
+  from \<sigma>_strat_R interpret \<sigma>_graph_R:
+    finite_graph_V_succ "Restr ?G\<sigma> R" "?V\<sigma> \<inter> R"
+    unfolding induced_subgraph_V_def
+    apply (unfold_locales; force?)
+    subgoal for v using R_game.ind_subgraph_succ[of v]
+      unfolding R_game.strategy_of_player_def R_game.strategy_of_def
+      using R_game_G\<sigma>_eq R_game_V\<sigma>_eq induced_subgraph_V_def
+      by clarsimp blast
+    done
+  (** There are no open vertices because every node has a successor in Z. *)
+  from \<open>R=Z\<close> step have "Ov = {}"
+    using R_game.succ by auto
   with step have Y'_def:
     "Y' = Y \<union> {U. bound_nt_bottom_SCC R Z \<sigma> U}"
-    by auto
-
-  have "\<exists>U. bound_nt_bottom_SCC R Z \<sigma> U"
+    by presburger
+  (** We show there exists a nontrivial bottom SCC in Z. *)
+  moreover have "\<exists>U. bound_nt_bottom_SCC R Z \<sigma> U"
   proof -
-    from \<open>R=Z\<close> R_game.tangle_attractor_strat[OF fin_T attr] have
-      \<sigma>_strat: "strategy_of (V_player \<alpha>) \<sigma>" and
-      \<sigma>_ran: "ran \<sigma> \<subseteq> Z" and
-      \<sigma>_closed: "(Restr ?G\<sigma> Z) `` Z \<subseteq> Z" and
-      \<sigma>_path_to_A: "\<forall>x\<in>Z. \<exists>y\<in>A. \<exists>xs. path (Restr ?G\<sigma> Z) x xs y"
-      unfolding restr_subgraph_V_player[OF R_valid_game]
-      unfolding restr_ind_subgraph[OF paritygame.axioms[OF R_valid_game]]
-      using restr_subgraph_strategy_of_player[OF R_valid_game]
-      by auto
-
-    then interpret \<sigma>_graph:
-      finite_graph_V_succ ?G\<sigma> ?V\<sigma>
-      unfolding strategy_of_def
-      apply unfold_locales
-      by (auto simp: finite_graph_V.E_in_V ind_subgraph_succ)
-
-    have \<sigma>_dom: "dom \<sigma> = V_player \<alpha> \<inter> Z"
-    proof
-      show "dom \<sigma> \<subseteq> V_player \<alpha> \<inter> Z"
-        using R_game.tangle_attractor_strat[OF fin_T attr]
-        unfolding restr_subgraph_V_player[OF R_valid_game] by simp
-    next
-      from \<open>R=Z\<close> \<open>R\<subseteq>V\<close> show "V_player \<alpha> \<inter> Z \<subseteq> dom \<sigma>"
-        using R_game.succ
-        using R_game.tangle_attractor_strat_in_dom_A[OF fin_T attr]
-        using R_game.tangle_attractor_strat_in_dom_not_A[OF fin_T attr]
-        unfolding restr_subgraph_V_player[OF R_valid_game]
-        by blast
-    qed
-
-    hence G\<sigma>_is_E_outside_Z: "Restr ?G\<sigma> (-Z) = Restr E (-Z)"
-      unfolding induced_subgraph_def E_of_strat_def
-      by blast
-
-    from \<sigma>_strat have "EV (E_of_strat \<sigma>) \<subseteq> ?V\<sigma>"
-      unfolding strategy_of_def induced_subgraph_V_def induced_subgraph_def E_of_strat_def
-      by auto
-
-    moreover have "dom \<sigma> \<subseteq> EV (E_of_strat \<sigma>)"
-      unfolding E_of_strat_def dom_def by force
-
-    ultimately have dom_in_V: "dom \<sigma> \<subseteq> ?V\<sigma>"
-      by auto
-
-    from \<open>R=Z\<close> R_game.tangle_attractor_strat[OF fin_T attr]
-    have \<sigma>_edges_in_Z: "E_of_strat \<sigma> \<subseteq> Restr E Z"
-      unfolding R_game.strategy_of_player_def R_game.strategy_of_def
-      by auto
-
-    from restr_ind_subgraph[OF paritygame.axioms[OF R_valid_game]]
-    have subgames_equal_in_Z: "R_game.induced_subgraph \<sigma> = Restr ?G\<sigma> Z"
-      by (simp add: \<open>R=Z\<close>)
-
-    have subgame_V_equal_in_Z:
-      "R_game.induced_subgraph_V \<sigma> = ?V\<sigma> \<inter> Z"
-    proof
-      show "R_game.induced_subgraph_V \<sigma> \<subseteq> ?V\<sigma> \<inter> Z"
-        unfolding R_game.induced_subgraph_V_def induced_subgraph_V_def
-        unfolding subgames_equal_in_Z by auto
-    next
-      show "?V\<sigma> \<inter> Z \<subseteq> R_game.induced_subgraph_V \<sigma>"
-      proof
-        fix x assume x_in_\<sigma>_V_Int_Z: "x \<in> ?V\<sigma> \<inter> Z"
-        hence "x \<in> Z" by auto
-
-        consider (in_dom) "x \<in> dom \<sigma>" | (notin_dom) "x \<notin> dom \<sigma>" by blast
-        thus "x \<in> R_game.induced_subgraph_V \<sigma>" proof cases
-          case in_dom
-          with \<sigma>_ran obtain y where
-            "y \<in> Z" "(x,y) \<in> E_of_strat \<sigma>"
-            unfolding E_of_strat_def ran_def by blast
-          hence "(x,y) \<in> Restr (R_game.induced_subgraph \<sigma>) Z"
-            unfolding subgames_equal_in_Z induced_subgraph_def
-            using \<sigma>_edges_in_Z by blast
-          thus ?thesis
-            unfolding R_game.induced_subgraph_V_def by force
-        next
-          case notin_dom
-          from \<open>x\<in>Z\<close> \<open>R\<subseteq>V\<close> \<open>R=Z\<close> obtain y where
-            "(x,y) \<in> Restr E Z"
-            using R_game.succ[of x] by blast
-          with \<open>R=Z\<close> have "(x,y) \<in> Restr (R_game.induced_subgraph \<sigma>) Z"
-            using R_game.ind_subgraph_notin_dom[OF _ notin_dom] by blast
-          thus ?thesis
-            unfolding R_game.induced_subgraph_V_def by force
-        qed
-      qed
-    qed
-
-    interpret \<sigma>_graph_Z:
-      finite_graph_V_succ "Restr ?G\<sigma> Z" "?V\<sigma> \<inter> Z"
-    proof (unfold_locales)
-      show "Restr ?G\<sigma> Z \<subseteq> (?V\<sigma> \<inter> Z) \<times> (?V\<sigma> \<inter> Z)"
-        using \<sigma>_graph.E_in_V by blast
-      show "finite (?V\<sigma> \<inter> Z)" by blast
-      show "\<And>v. v \<in> ?V\<sigma> \<inter> Z \<Longrightarrow> Restr ?G\<sigma> Z `` {v} \<noteq> {}"
-        using \<open>R=Z\<close> R_game.ind_subgraph_succ \<sigma>_edges_in_Z
-        using subgame_V_equal_in_Z subgames_equal_in_Z by blast
-    qed
-
-    from \<open>R=Z\<close> interpret \<sigma>_graph_R:
-      finite_graph_V_succ "Restr ?G\<sigma> R" "?V\<sigma> \<inter> R"
-      using \<sigma>_graph_Z.finite_graph_V_succ_axioms by blast
-
-
-    from \<open>R\<noteq>{}\<close> \<open>R\<subseteq>V\<close> \<open>R=Z\<close> have "Restr E Z `` Z \<noteq> {}"
-      using R_game.succ by blast
-
-    from \<open>A\<noteq>{}\<close> obtain a where "a \<in> A" by blast
-    with \<open>A\<subseteq>Z\<close> \<open>R=Z\<close> have "a \<in> R" by blast
-    have "a \<in> induced_subgraph_V \<sigma> \<inter> Z"
-    proof -
-      consider (dom) "a \<in> dom \<sigma>" | (not_dom) "a \<notin> dom \<sigma>" by blast
-      thus ?thesis proof cases
-        case dom with \<open>A\<subseteq>Z\<close> \<open>a\<in>A\<close> dom_in_V
-        show ?thesis  by auto
-      next
-        case not_dom with \<open>a\<in>R\<close> show ?thesis
-          unfolding induced_subgraph_V_def
-          using ind_subgraph_notin_dom[OF _ not_dom]
-          using R_game.succ[of a]
-          apply (clarsimp simp add: Int_absorb1[OF \<open>R\<subseteq>V\<close>])
-          using image_iff \<open>R=Z\<close> by fastforce
-      qed
-    qed
-    from \<sigma>_graph_Z.cycle_always_exists[OF this]
-    obtain y ys where cycle: "cycle (Restr ?G\<sigma> Z) y ys"
-      unfolding reachable_cycle_def by blast
-    hence "set ys \<noteq> {}" by auto
-    have ys_conn: "strongly_connected (Restr (Restr ?G\<sigma> Z) (set ys)) (set ys)"
-      using cycle_strongly_connected[OF cycle] by blast
-
-    from \<sigma>_graph_R.nt_bottom_SCC_ex obtain U where
-      "\<sigma>_graph_R.nt_bottom_SCC U"
-      using \<open>a \<in> induced_subgraph_V \<sigma> \<inter> Z\<close> \<open>R=Z\<close> by blast
-
-    thus ?thesis
-      using \<sigma>_graph_R.nt_bottom_SCC_in_V \<open>R=Z\<close> by blast
+    (** The subgraph of \<sigma> in R has nodes in it. *)
+    from \<sigma>_strat_R \<open>R\<subseteq>V\<close> \<open>R\<noteq>{}\<close> have "?V\<sigma> \<inter> R \<noteq> {}"
+      unfolding R_game.strategy_of_player_def
+      using R_game.strategy_of_in_E[of _ \<sigma>]
+      using R_game.ind_subgraph_V_notempty[of \<sigma>]
+      unfolding R_game_V\<sigma>_eq by blast
+    (** This means there exists a nontrivial bottom SCC. *)
+    with \<open>R=Z\<close> show ?thesis
+      using \<sigma>_graph_R.nt_bottom_SCC_ex
+      using \<sigma>_graph_R.nt_bottom_SCC_in_V by blast
   qed
-  thus ?case
-    unfolding Y'_def by simp
+  ultimately show ?case by simp
 qed
 
-lemma search_step_rtranclp_last:
+(** If the initial R is nonempty, and the resulting R' of the reflexive
+    transitive closure of search_step is empty, then the obtained Y' is not empty. *)
+lemma search_step_rtranclp_last_R'_empty:
   "\<lbrakk>search_step\<^sup>*\<^sup>* (R,Y) (R',Y'); search_I (R,Y); R \<noteq> {}; R' = {}\<rbrakk> \<Longrightarrow> Y' \<noteq> {}"
   apply (induction rule: rtranclp_induct2)
-  by (auto simp: search_step_last search_step_rtranclp_preserves_I)
+  by (auto simp: search_step_last_R'_empty search_step_rtranclp_preserves_I)
 
-lemma search_step_nonempty_R:
+(** If we have a nonempty R that is a valid subgame, then search gives a nonempty Y. *)
+lemma search_nonempty_R:
   "\<lbrakk>search R Y; valid_subgame R; R \<noteq> {}\<rbrakk> \<Longrightarrow> Y \<noteq> {}"
   unfolding search_def
-  using search_step_rtranclp_last search_I_base by simp
+  using search_step_rtranclp_last_R'_empty search_I_base by simp
 
-lemma search_step_notempty[simp]: "\<not>search_step ({},Y) (R',Y')"
-  by (simp add: search_step.simps)
-
-lemma search_step_rtranclp_empty_R: "\<lbrakk>search_step\<^sup>*\<^sup>* (R,Y) (R',Y'); R = {}\<rbrakk> \<Longrightarrow> Y = Y'"
-  by (induction rule: converse_rtranclp_induct2) auto
-
-lemma search_empty_R:
-  "\<lbrakk>search {} Y\<rbrakk> \<Longrightarrow> Y = {}"
-  unfolding search_def
-  using search_step_rtranclp_empty_R by blast
 
 subsection \<open>Correctness\<close>
-(** If we end with an empty region, then we have a finite, non-empty Y containing new tangles that
-    were not included in T before, as specified by our invariant. *)
-lemma search_I_correct:
-  "search_I ({},Y) \<Longrightarrow> finite Y \<and> (\<forall>U \<in> Y. \<exists>\<alpha>. tangle \<alpha> U \<and> U \<notin> T)"
-  unfolding search_I_def by simp
-
 (** If the initial R is a valid subgame, then search gives us a finite, non-empty Y that contains
     new tangles that were not included in T before. *)
 theorem search_correct:
   "\<lbrakk>valid_subgame R; search R Y\<rbrakk>
-    \<Longrightarrow> finite Y \<and> (R \<noteq> {} \<longleftrightarrow> Y \<noteq> {}) \<and> (\<forall>U \<in> Y. \<exists>\<alpha>. tangle \<alpha> U \<and> U \<notin> T)"
+    \<Longrightarrow> finite Y \<and> (R \<noteq> {} \<longleftrightarrow> Y \<noteq> {}) \<and> (\<forall>U \<in> Y. \<exists>\<alpha>. tangle \<alpha> U)"
   using search_I_correct[OF search_preserves_I[OF _ search_I_base]]
-  apply (safe; clarsimp)
-  subgoal using search_step_nonempty_R by fast
-  subgoal using search_empty_R by fastforce
-  done
+  using search_nonempty_R search_empty_R by fast
 
 
 section \<open>Termination\<close>
